Sorting/Sort.v
@@ -2,55 +2,57 @@ Add Rec LoadPath "/home/zeimer/Code/Coq".
 
 Require Export RCCBase.
 
-(*Require Export Sorting.Perm_generalized.*)
 Require Export Sorting.Perm.
 
-Inductive sorted (A : LinDec) : list A -> Prop :=
-    | sorted0 : sorted A []
-    | sorted1 : forall x : A, sorted A [x]
-    | sorted2 : forall (x y : A) (l : list A),
-        x ≤ y -> sorted A (y :: l) -> sorted A (x :: y :: l).
+Inductive Sorted (A : LinDec) : list A -> Prop :=
+    | Sorted0 : Sorted A []
+    | Sorted1 : forall x : A, Sorted A [x]
+    | Sorted2 : forall (x y : A) (l : list A),
+        x ≤ y -> Sorted A (y :: l) -> Sorted A (x :: y :: l).
 
-Hint Constructors sorted.
+Hint Constructors Sorted.
 
 Class Sort (A : LinDec) : Type :=
 {
     sort :> list A -> list A;
-    sort_sorted :
-      forall l : list A, sorted A (sort l);
-    sort_perm :
-      forall l : list A, perm A l (sort l);
+    Sorted_sort :
+      forall l : list A, Sorted A (sort l);
+(*    sort_perm :
+      forall l : list A, perm A l (sort l);*)
+    Permutation_sort :
+      forall l : list A, Permutation (sort l) l
 }.
-
-Lemma Permutation_sort :
-  forall (A : LinDec) (s : Sort A) (l : list A), Permutation (sort l) l.
-Proof.
-  intros. apply perm_Permutation. rewrite <- sort_perm. reflexivity.
-Qed.
 
 Coercion sort : Sort >-> Funclass.
 
-(* Lemmas about [sorted]. *)
+Lemma sort_perm :
+  forall (A : LinDec) (s : Sort A) (l : list A),
+    perm A l (sort l).
+Proof.
+  intros. apply Permutation_perm. rewrite Permutation_sort. reflexivity.
+Qed.
 
-Theorem sorted_tail :
+(* Lemmas about [Sorted]. *)
+
+Theorem Sorted_tail :
   forall (A : LinDec) (h : A) (t : list A),
-    sorted A (h :: t) -> sorted A t.
+    Sorted A (h :: t) -> Sorted A t.
 Proof.
   inversion 1; auto.
 Defined.
 
-Theorem sorted_head :
+Theorem Sorted_head :
   forall (A : LinDec) (x y : A) (l : list A),
-    sorted A (x :: y :: l) -> x ≤ y.
+    Sorted A (x :: y :: l) -> x ≤ y.
 Proof.
   inversion 1. assumption.
 Qed.
 
-Lemma sorted_app_all :
+Lemma Sorted_app_all :
   forall (A : LinDec) (l : list A) (h : A) (t : list A),
-    sorted A l -> sorted A (h :: t) ->
+    Sorted A l -> Sorted A (h :: t) ->
     (forall x : A, In x l -> leq x h) ->
-      sorted A (l ++ h :: t).
+      Sorted A (l ++ h :: t).
 Proof.
   induction l as [| h t]; simpl; intros.
     assumption.
@@ -59,29 +61,29 @@ Proof.
         eapply (H1 h); eauto.
         assumption.
       rewrite <- app_comm_cons. constructor.
-        eapply sorted_head. eassumption.
+        eapply Sorted_head. eassumption.
         apply IHt.
-          apply sorted_tail with h. assumption.
+          apply Sorted_tail with h. assumption.
           assumption.
           intros. apply H1. right. assumption.
 Qed.
 
-Lemma sorted_app :
+Lemma Sorted_app :
   forall (A : LinDec) (l1 l2 : list A),
-    sorted A l1 -> sorted A l2 ->
+    Sorted A l1 -> Sorted A l2 ->
       (forall x y : A, In x l1 -> In y l2 -> x ≤ y) ->
-        sorted A (l1 ++ l2).
+        Sorted A (l1 ++ l2).
 Proof.
   destruct l2 as [| h2 t2]; cbn; intros.
     rewrite app_nil_r. assumption.
-    apply sorted_app_all; auto.
+    apply Sorted_app_all; auto.
 Qed.
 
-Hint Resolve sorted_head sorted_tail sorted_app_all.
+Hint Resolve Sorted_head Sorted_tail Sorted_app_all.
 
-Lemma sorted_cons :
+Lemma Sorted_cons :
   forall (A : LinDec) (h : A) (t : list A),
-    (forall x : A, In x t -> h ≤ x) -> sorted A t -> sorted A (h :: t).
+    (forall x : A, In x t -> h ≤ x) -> Sorted A t -> Sorted A (h :: t).
 Proof.
   inversion 2; subst.
     auto.
@@ -91,36 +93,36 @@ Proof.
       constructor; auto.
 Qed.
 
-Lemma sorted_mid :
+Lemma Sorted_mid :
   forall (A : LinDec) (x y : A) (l : list A),
-    sorted A (x :: y :: l) -> sorted A (x :: l).
+    Sorted A (x :: y :: l) -> Sorted A (x :: l).
 Proof.
   destruct l.
     auto.
     intros. constructor.
-      assert (x ≤ y) by (apply sorted_head in H; auto).
-        apply sorted_tail in H.
-        assert (y ≤ c) by (apply sorted_head in H; auto).
+      assert (x ≤ y) by (apply Sorted_head in H; auto).
+        apply Sorted_tail in H.
+        assert (y ≤ c) by (apply Sorted_head in H; auto).
         eapply leq_trans; eauto.
-      do 2 eapply sorted_tail. eassumption.
+      do 2 eapply Sorted_tail. eassumption.
 Qed.
 
-Lemma sorted_cons_conv :
+Lemma Sorted_cons_conv :
   forall (A : LinDec) (h : A) (t : list A),
-    sorted A (h :: t) -> forall x : A, In x t -> h ≤ x.
+    Sorted A (h :: t) -> forall x : A, In x t -> h ≤ x.
 Proof.
   induction t as [| h' t'].
     inversion 2.
     intros. inversion H0; subst.
-      apply sorted_head in H. assumption.
+      apply Sorted_head in H. assumption.
       apply IHt'.
-        apply sorted_mid in H. assumption.
+        apply Sorted_mid in H. assumption.
         assumption.
 Qed.
 
-Lemma sorted_cons_conv' :
+Lemma Sorted_cons_conv' :
   forall (A : LinDec) (h : A) (t : list A),
-    sorted A (h :: t) -> forall x : A, In x (h :: t) -> h ≤ x.
+    Sorted A (h :: t) -> forall x : A, In x (h :: t) -> h ≤ x.
 Proof.
   induction t as [| h' t'].
     inversion 2; subst; dec.
@@ -129,25 +131,25 @@ Proof.
       inversion H6; subst.
         assumption.
         apply IHt'.
-          eapply sorted_mid; eauto.
+          eapply Sorted_mid; eauto.
           right. assumption.
 Qed.
 
 (* Moved from TrichQuicksortSpec.v *)
 
-Lemma repeat_sorted :
+Lemma Sorted_repeat :
   forall (A : LinDec) (x : A) (n : nat),
-    sorted A (repeat x n).
+    Sorted A (repeat x n).
 Proof.
   induction n as [| n']; cbn.
     constructor.
     destruct n'; cbn; constructor; auto.
 Qed.
 
-Lemma filter_eqb_sorted :
+Lemma Sorted_filter_eqb :
   forall (A : LinDec) (x : A) (l : list A),
-    sorted A (filter (fun x' : A => x' =? x) l).
+    Sorted A (filter (fun x' : A => x' =? x) l).
 Proof.
   intros. destruct (filter_eqb_repeat A x l) as [n H].
-  rewrite H. apply repeat_sorted.
+  rewrite H. apply Sorted_repeat.
 Qed.
